Co-total of maximal, extends to allowable of total
Signed-off-by: thirdsgames <thirdsgames2018@gmail.com>

src/phase2/freedom_of_action.lean
@@ -209,6 +209,9 @@ def spec.total {α : type_index} (σ : spec α) : Prop := σ.domain = set.univ
 /-- A specification is co-total if it specifies where every element in its codomain came from. -/
 def spec.co_total {α : type_index} (σ : spec α) : Prop := σ.range = set.univ
 
+lemma spec.co_total_of_inv_total {α : type_index} (σ : spec α) :
+  σ⁻¹.total → σ.co_total := sorry
+
 lemma spec.total_1_1_restriction {α β : type_index} (σ : spec α) (A : path (α : type_index) β) :
   (σ.total → (σ.lower A).total) ∧ (σ.co_total → (σ.lower A).co_total) :=
 begin
@@ -411,7 +414,6 @@ namespace spec
 
 variable (B)
 
-
 /-!
 We now set out the allowability conditions for specifications of permutations.
 These are collected in the structure `allowable_spec`, which may be treated as a proposition.
@@ -537,8 +539,50 @@ end spec
 
 variable (B)
 
+namespace spec
+section has_inv
+
+variables {σ : spec B}
+
+lemma inv_one_to_one (hσ : σ.allowable_spec B) : σ⁻¹.one_to_one B := sorry
+
+lemma inv_atom_cond (hσ : σ.allowable_spec B) : ∀ L C, σ⁻¹.atom_cond B L C := sorry
+
+lemma inv_near_litter_cond (hσ : σ.allowable_spec B) : ∀ N C, σ⁻¹.near_litter_cond B N C := sorry
+
+lemma inv_flexible_cond (hσ : σ.allowable_spec B) : σ⁻¹.flexible_cond B := sorry
+
+lemma inv_domain_closed (hσ : σ.allowable_spec B) : σ⁻¹.domain.support_closed B := sorry
+
+lemma inv_range_closed (hσ : σ.allowable_spec B) : σ⁻¹.range.support_closed B := sorry
+
+-- Note: the non-flexible conditions can't be worked on yet, until allowable.lean compiles.
+
+lemma inv_non_flexible_cond (hσ : σ.allowable_spec B) : σ⁻¹.non_flexible_cond B := sorry
+
+lemma inv_inv_non_flexible_cond (hσ : σ.allowable_spec B) : σ⁻¹⁻¹.non_flexible_cond B := sorry
+
+/-- The inverse of an allowable specification is allowable. -/
+lemma inv_allowable (σ : spec B) (hσ : σ.allowable_spec B) :
+  σ⁻¹.allowable_spec B := {
+  one_to_one := inv_one_to_one B hσ,
+  atom_cond := inv_atom_cond B hσ,
+  near_litter_cond := inv_near_litter_cond B hσ,
+  flexible_cond := inv_flexible_cond B hσ,
+  domain_closed := inv_domain_closed B hσ,
+  range_closed := inv_range_closed B hσ,
+  non_flexible_cond := inv_non_flexible_cond B hσ,
+  inv_non_flexible_cond := inv_inv_non_flexible_cond B hσ,
+}
+
+end has_inv
+end spec
+
 /-- An *allowable partial permutation* is a specification that is allowable as defined above. -/
 def allowable_partial_perm := {σ : spec B // σ.allowable_spec B}
+
+instance allowable_partial_perm.has_inv : has_inv (allowable_partial_perm B) :=
+⟨λ σ, ⟨σ.val⁻¹, σ.val.inv_allowable B σ.property⟩⟩
 
 /-! We prove the restriction lemma: if `σ` is a partial allowable permutation, then so is `σ`
 restricted to a lower path `A`. The proof should be mostly straightforward. The non-trivial bit is
@@ -576,7 +620,8 @@ lemma lower_non_flexible_cond (hσ : σ.allowable_spec B) :
 lemma lower_inv_non_flexible_cond (hσ : σ.allowable_spec B) :
   (σ.lower A)⁻¹.non_flexible_cond (le_index.mk β (path.comp B.path A)) := sorry
 
-lemma lower_allowable (hσ : σ.allowable_spec B) :
+lemma lower_allowable (σ : spec B) (hσ : σ.allowable_spec B)
+  ⦃β : Λ⦄ (A : path (B : type_index) β) (hβ : (β : type_index) < B) :
   (σ.lower A).allowable_spec (le_index.mk β (path.comp B.path A)) := {
   one_to_one := lower_one_to_one B A hσ,
   atom_cond := lower_atom_cond B A hσ,
@@ -622,7 +667,7 @@ We now define a preorder on partial allowable permutations.
 * `σ` is a subset of `ρ`;
 * if `ρ` has any new flexible litter, then it has all (in both domain and range);
 * within each litter, if `ρ.domain` has any new atom, then it must have all
-    atoms in that litter (and hence must also have the litter).
+    atoms in that litter (and hence must also have the litter), and dually for the range.
 
 Note that the second condition is exactly the condition in `spec.flexible_cond.all`.
 -/
@@ -633,10 +678,14 @@ structure perm_le (σ ρ : allowable_partial_perm B) : Prop :=
   (hρ : (⟨sum.inr ⟨L.to_near_litter, N⟩, A⟩ : binary_condition B) ∈ ρ.val) :
   (∀ L A, flexible L A → (⟨sum.inr L.to_near_litter, A⟩ : support_condition B) ∈ ρ.val.domain) ∧
   (∀ L A, flexible L A → (⟨sum.inr L.to_near_litter, A⟩ : support_condition B) ∈ ρ.val.range))
-(all_atoms (a b : atom) (L : litter) (ha : a ∈ litter_set L) (A : extended_index B)
+(all_atoms_domain (a b : atom) (L : litter) (ha : a ∈ litter_set L) (A : extended_index B)
   (hσ : (⟨sum.inl ⟨a, b⟩, A⟩ : binary_condition B) ∉ σ.val)
   (hρ : (⟨sum.inl ⟨a, b⟩, A⟩ : binary_condition B) ∈ ρ.val) :
   ∀ c ∈ litter_set L, ∃ d, (⟨sum.inl ⟨c, d⟩, A⟩ : binary_condition B) ∈ ρ.val)
+(all_atoms_range (a b : atom) (L : litter) (ha : b ∈ litter_set L) (A : extended_index B)
+  (hσ : (⟨sum.inl ⟨a, b⟩, A⟩ : binary_condition B) ∉ σ.val)
+  (hρ : (⟨sum.inl ⟨a, b⟩, A⟩ : binary_condition B) ∈ ρ.val) :
+  ∀ c ∈ litter_set L, ∃ d, (⟨sum.inl ⟨d, c⟩, A⟩ : binary_condition B) ∈ ρ.val)
 
 instance has_le : has_le (allowable_partial_perm B) := ⟨perm_le B⟩
 
@@ -645,14 +694,16 @@ instance has_le : has_le (allowable_partial_perm B) := ⟨perm_le B⟩
 lemma extends_refl (σ : allowable_partial_perm B) : σ ≤ σ :=
 ⟨set.subset.rfl,
  λ _ _ _ _ h1 h2, by cases h1 h2,
+ λ _ _ _ _ _ h1 h2, by cases h1 h2,
  λ _ _ _ _ _ h1 h2, by cases h1 h2⟩
 
 lemma extends_trans (ρ σ τ : allowable_partial_perm B)
   (h₁ : ρ ≤ σ) (h₂ : σ ≤ τ) : ρ ≤ τ :=
 begin
-  obtain ⟨hsub, hflx, hatom⟩ := h₁,
-  obtain ⟨hsub', hflx', hatom'⟩ := h₂,
-  refine ⟨hsub.trans hsub', λ L N A hLA hnin hin, _, λ a b L hab A hnin hin, _⟩,
+  obtain ⟨hsub, hflx, hatom_domain, hatom_range⟩ := h₁,
+  obtain ⟨hsub', hflx', hatom_domain', hatom_range'⟩ := h₂,
+  refine ⟨hsub.trans hsub', λ L N A hLA hnin hin, _,
+    λ a b L hab A hnin hin, _, λ a b L hab A hnin hin, _⟩,
   { by_cases (sum.inr (L.to_near_litter, N), A) ∈ σ.val,
     { split; intros l a hla,
       { exact set.image_subset binary_condition.domain hsub' ((hflx L N A hLA hnin h).1 l a hla) },
@@ -660,9 +711,14 @@ begin
     { exact hflx' L N A hLA h hin } },
   { by_cases (sum.inl (a, b), A) ∈ σ.val,
     { intros c hc,
-      obtain ⟨d, hd⟩ := hatom a b L hab A hnin h c hc,
+      obtain ⟨d, hd⟩ := hatom_domain a b L hab A hnin h c hc,
       refine ⟨d, hsub' hd⟩ },
-    { exact hatom' a b L hab A h hin } }
+    { exact hatom_domain' a b L hab A h hin } },
+  { by_cases (sum.inl (a, b), A) ∈ σ.val,
+    { intros c hc,
+      obtain ⟨d, hd⟩ := hatom_range a b L hab A hnin h c hc,
+      refine ⟨d, hsub' hd⟩ },
+    { exact hatom_range' a b L hab A h hin } },
 end
 
 instance preorder : preorder (allowable_partial_perm B) := {
@@ -670,6 +726,12 @@ instance preorder : preorder (allowable_partial_perm B) := {
   le_refl := extends_refl B,
   le_trans := extends_trans B,
 }
+
+/-- A condition required later. -/
+lemma inv_le (σ τ : allowable_partial_perm B) : σ ≤ τ → σ⁻¹ ≤ τ⁻¹ := sorry
+
+/-- Inverses are involutive. -/
+@[simp] lemma inv_inv (σ : allowable_partial_perm B) : σ⁻¹⁻¹ = σ := sorry
 
 section zorn_setup
 
@@ -791,25 +853,36 @@ lemma total_of_maximal (σ : allowable_partial_perm B) (hσ : ∀ ρ ≥ σ, ρ 
 
 /-- Any maximal allowable partial permutation under `≤` is co-total. -/
 lemma co_total_of_maximal (σ : allowable_partial_perm B) (hσ : ∀ ρ ≥ σ, ρ = σ)
-  (foa : ∀ (B : lt_index α), freedom_of_action (B : le_index α)) : σ.val.co_total := sorry
+  (foa : ∀ (B : lt_index α), freedom_of_action (B : le_index α)) : σ.val.co_total :=
+begin
+  refine spec.co_total_of_inv_total σ.val (total_of_maximal B σ⁻¹ _ foa),
+  intros ρ hρ,
+  convert congr_arg has_inv.inv (hσ ρ⁻¹ _),
+  rw inv_inv,
+  convert inv_le B σ⁻¹ ρ hρ,
+  rw inv_inv,
+end
 
 /-- Any allowable partial permutation extends to an allowable permutation at level `α`, given that
 it is total and co-total. This is `total-allowable-partial-perm-actual` in the blueprint. -/
 lemma extends_to_allowable_of_total (σ : allowable_partial_perm ⟨α, path.nil⟩)
   (hσ₁ : σ.val.total) (hσ₂ : σ.val.co_total)
   (foa : ∀ (B : lt_index α), freedom_of_action (B : le_index α)) :
-  ∃ (π : allowable_path ⟨α, path.nil⟩), (allowable_path_to_struct_perm _ π).satisfies σ.val := sorry
-
-noncomputable def to_allowable_of_total (σ : allowable_partial_perm ⟨α, path.nil⟩)
-  (hσ₁ : σ.val.total) (hσ₂ : σ.val.co_total)
-  (foa : ∀ (B : lt_index α), freedom_of_action (B : le_index α)) : allowable_path ⟨α, path.nil⟩ :=
-Exists.some $ extends_to_allowable_of_total σ hσ₁ hσ₂ foa
-
-lemma to_allowable_of_total_spec (σ : allowable_partial_perm ⟨α, path.nil⟩)
-  (hσ₁ : σ.val.total) (hσ₂ : σ.val.co_total)
-  (foa : ∀ (B : lt_index α), freedom_of_action (B : le_index α)) :
-  (allowable_path_to_struct_perm _  $ σ.to_allowable_of_total hσ₁ hσ₂ foa).satisfies σ.val :=
-Exists.some_spec $ extends_to_allowable_of_total σ hσ₁ hσ₂ foa
+  ∃ (π : allowable_path ⟨α, path.nil⟩), (allowable_path_to_struct_perm _ π).satisfies σ.val :=
+begin
+  have lower_allowable_spec :
+    ∀ (B : proper_lt_index α), (σ.val.lower B.path).allowable_spec (B : le_index α),
+  { intro B,
+    have := lower_allowable ⟨α, path.nil⟩ σ.val σ.property B.path
+      (coe_lt_coe.mpr (B.index_lt.trans_le (coe_le_coe.mp $ le_of_path B.path'))),
+    rw path.nil_comp at this,
+    exact this, },
+  have exists_lower_allowable : ∀ (B : proper_lt_index α), ∃ (π : allowable_path (B : le_index α)),
+    (allowable_path_to_struct_perm (B : le_index α) π).satisfies (σ.val.lower B.path) :=
+    λ B, foa B ⟨σ.val.lower B.path, lower_allowable_spec B⟩,
+  -- We need allowable.lean to compile for the rest of this proof.
+  sorry
+end
 
 end allowable_partial_perm
 
